src/tls/Extract1.ODH.fst
@@ -7,7 +7,7 @@ open Idx
 open Pkg.Tree
 open KDF // avoid?
 
-module MM = FStar.Monotonic.Map
+module MDM = FStar.Monotonic.DependentMap
 
 open Extract1.PRF // for now
 
@@ -23,7 +23,7 @@ let there = Mem.tls_tables_region
 // (i,gY).
 // The table exists when [Flags.ideal_KDF], a precondition for [flag_odh]
 
-// We need a variant of FStar.Monotonic.Map that enables monotonic updates to
+// Wen need a variant of FStar.Monotonic.Map that enables monotonic updates to
 // each entry. We used nested ones to re-use existing libraries, but
 // may instead invest is a custom library.
 //
@@ -46,17 +46,17 @@ type peer_instance (#x:odhid) (iy:peer_index x) =
   secret d u (Derive (dfst iy) "" (ExtractDH (IDH x (dsnd iy)))))
 
 let peer_table (x:odhid): Type0 =
-  MM.t there (peer_index x) (peer_instance #x) (fun _ -> True)
-type odh_table = MM.t there odhid peer_table (fun _ -> True)
+  MDM.t there (peer_index x) (peer_instance #x) (fun _ -> True)
+type odh_table = MDM.t there odhid peer_table (fun _ -> True)
 
 let odh_state : (if model then odh_table else unit) =
-  if model then MM.alloc #there #odhid #peer_table #(fun _ -> True)
+  if model then MDM.alloc #there #odhid #peer_table #(fun _ -> True)
   else ()
 
 type odh_fresh (i:odhid) (h:mem) =
   (if model then
     let log : odh_table = odh_state in
-    MM.fresh log i h
+    MDM.fresh log i h
   else True)
 
 let lemma_fresh_odh (i:CommonDH.dhi) (h:mem)
@@ -70,15 +70,15 @@ let lemma_fresh_odh_framing (i:CommonDH.dhi) (h0:mem) (h1:mem)
 type odh_defined (i:odhid) =
   (if model then
     let log : odh_table = odh_state in
-    witnessed (MM.defined log i)
+    witnessed (MDM.defined log i)
   else True)
 
 type odhr_fresh (#i:odhid) (r:peer_index i) (h:mem) =
   (if model then
     let log : odh_table = odh_state in
-    (match MM.sel (sel h log) i with
+    (match MDM.sel (sel h log) i with
     | Some t ->
-      (match MM.sel (sel h t) r with
+      (match MDM.sel (sel h t) r with
       | None -> True
       | _ -> False)
     | _ -> False)
@@ -111,13 +111,13 @@ let odh_init g =
     let i : CommonDH.dhi = (| g, CommonDH.ipubshare x |) in
     lemma_fresh_odh i h0;
     lemma_fresh_odh_framing i h0 h1;
-    assert(MM.sel (sel h1 log) i == None);
-    let peers = alloc tls_tables_region <: peer_table i in //17-11-22   MM.alloc #there #(peer_index i) #(peer_instance #i) #(fun _ -> True) in
+    assert(MDM.sel (sel h1 log) i == None);
+    let peers = alloc tls_tables_region <: peer_table i in //17-11-22   MDM.alloc #there #(peer_index i) #(peer_instance #i) #(fun _ -> True) in
     let h2 = get () in
-    assume(MM.sel (sel h2 log) i == None); // FIXME allocate peers somewhere else !!
-    MM.extend log i peers;
-    assume(stable_on_t log (MM.defined log i));
-    mr_witness log (MM.defined log i)
+    assume(MDM.sel (sel h2 log) i == None); // FIXME allocate peers somewhere else !!
+    MDM.extend log i peers;
+    assume(stable_on_t log (MDM.defined log i));
+    mr_witness log (MDM.defined log i)
    end;
   x
 
@@ -143,13 +143,13 @@ private let register_odh (i:regid) (gX:CommonDH.dhi) (gY:CommonDH.dhr gX)
   let j = Derive i "" ctx in // N.B. this is the only case where i can be corrupt and j honest
   let hlog : i_honesty_table = honesty_table in
   recall hlog;
-  match MM.lookup hlog j with
+  match MDM.lookup hlog j with
   | None ->
     let m = !hlog in
-    assume(honesty_invariant (MM.upd m j true)); // Sepcial case: honest IDH
-    MM.extend hlog j true;
-    MM.contains_stable hlog j true;
-    mr_witness hlog (MM.contains hlog j true); j
+    assume(honesty_invariant (MDM.upd m j true)); // Sepcial case: honest IDH
+    MDM.extend hlog j true;
+    MDM.contains_stable hlog j true;
+    mr_witness hlog (MDM.contains hlog j true); j
   | Some b -> j
 
 val odh_test:
@@ -196,9 +196,9 @@ let odh_test #d #u #i a s gX =
   let h2 = get() in
   assume(odhr_fresh j' h2); // TODO framing of KDF
   let t: odh_table = odh_state in
-  testify(MM.defined t gX);
-  let peers = Some?.v (MM.lookup t gX) in
-  MM.extend peers j' k;
+  testify(MDM.defined t gX);
+  let peers = Some?.v (MDM.lookup t gX) in
+  MDM.extend peers j' k;
   (| j' , k |)
 
 unfold let idh_of (#g:CommonDH.group) (x:CommonDH.ikeyshare g) (gY:CommonDH.rshare g (CommonDH.ipubshare x)) =
