src/tls/IdNonce.fst
@@ -9,7 +9,7 @@ open TLSConstants
 open TLSInfo
 
 module N=Nonce
-module MM = FStar.Monotonic.DependentMap
+module MDM = FStar.Monotonic.DependentMap
 module HS = FStar.HyperStack
 module HST = FStar.HyperStack.ST
 
@@ -19,28 +19,28 @@ type n_id (n:random) = i:id{nonce_of_id i = n}
 
 //nonce_id_table:
 //  A monotone, injective partial map in the tls_tables_region, from random to rid
-let nonce_id_table : MM.t tls_tables_region random n_id (fun x -> True) =
-  MM.alloc ()
+let nonce_id_table : MDM.t tls_tables_region random n_id (fun x -> True) =
+  MDM.alloc ()
 
-let id_of_nonce (n:random) (i:n_id n) = HST.witnessed (MM.contains nonce_id_table n i)
+let id_of_nonce (n:random) (i:n_id n) = HST.witnessed (MDM.contains nonce_id_table n i)
 
 let insert n i =
   HST.recall nonce_id_table;
-  MM.extend nonce_id_table n i
+  MDM.extend nonce_id_table n i
 
 val lookup: n:random -> ST (option (n_id n))
   (requires (fun h -> True))
   (ensures (fun h0 idopt h1 ->
     h0==h1 /\
     (match idopt with
-     | None -> MM.fresh nonce_id_table n h0
-     | Some i -> MM.contains nonce_id_table n i h0 /\
+     | None -> MDM.fresh nonce_id_table n h0
+     | Some i -> MDM.contains nonce_id_table n i h0 /\
                 id_of_nonce n i)))
-let lookup n = MM.lookup nonce_id_table n
+let lookup n = MDM.lookup nonce_id_table n
 
 val injectivity : n:random -> m:random -> i:n_id n -> j:n_id m ->  ST unit
   (requires (fun h -> i=!=j /\ id_of_nonce n i /\ id_of_nonce m j))
   (ensures (fun h0 _ h1 -> n<>m))
 let injectivity n m i j =
-  HST.testify (MM.contains nonce_id_table n i);
-  HST.testify (MM.contains nonce_id_table m j)
+  HST.testify (MDM.contains nonce_id_table n i);
+  HST.testify (MDM.contains nonce_id_table m j)
