src/tls/MasterSecret.fst
@@ -9,7 +9,7 @@ open FStar.HyperStack
 
 module AE = StreamAE
 module DM = FStar.DependentMap
-module MM = FStar.Monotonic.DependentMap
+module MDM = FStar.Monotonic.DependentMap
 module HS = FStar.HyperStack
 module HST = FStar.HyperStack.ST
 module N = Nonce
@@ -28,27 +28,27 @@ let writer (i:AE.id) = w:AE.writer i{
 
 // A partial map from i:id to w:writer i is region_injective
 // if it maps distinct ids to writers with distinct regions
-let region_injective (m:MM.partial_dependent_map AE.id writer) =
+let region_injective (m:MDM.partial_dependent_map AE.id writer) =
   forall i1 i2.{:pattern (DM.sel m i1); (DM.sel m i2)}
        i1=!=i2 ==> (match DM.sel m i1, DM.sel m i2 with
                           | Some w1, Some w2 -> w1.region <> w2.region
                           | _ -> True)
 
-let ms_tab : MM.t tls_tables_region AE.id writer region_injective =
-  MM.alloc ()
+let ms_tab : MDM.t tls_tables_region AE.id writer region_injective =
+  MDM.alloc ()
 
 //A region is fresh if no nonce is associated with it
 let fresh_in_ms_tab (r:rgn) (h:mem) =
-  forall i. match MM.sel (HS.sel h ms_tab) i with
+  forall i. match MDM.sel (HS.sel h ms_tab) i with
        | Some w -> w.region <> r
        | None -> True
 
-private let id_rgns_witnessed (m:MM.map AE.id writer) =
-    forall (i:AE.id{Some? (MM.sel m i)}). HST.witnessed (HST.region_contains_pred ((Some?.v (MM.sel m i)).region))
+private let id_rgns_witnessed (m:MDM.map AE.id writer) =
+    forall (i:AE.id{Some? (MDM.sel m i)}). HST.witnessed (HST.region_contains_pred ((Some?.v (MDM.sel m i)).region))
 
 private let contains_id_rgns (h:mem) =
     let m = HS.sel h ms_tab in
-    forall (i:AE.id{Some? (MM.sel m i)}). Map.contains h.h ((Some?.v (MM.sel m i)).region)
+    forall (i:AE.id{Some? (MDM.sel m i)}). Map.contains h.h ((Some?.v (MDM.sel m i)).region)
 
 
 (* private val all_ms_tab_regions_exists: unit -> ST unit //would be good to make such stateful lemmas STTot, once we have it; a bit loose for now *)
@@ -78,20 +78,20 @@ let derive (r:rgn) (i:AE.id)
            /\ modifies (Set.singleton tls_tables_region) h0 h1 //modifies at most the tls_tables region
            /\ HS.modifies_ref tls_tables_region (Set.singleton (as_addr ms_tab_as_hsref)) h0 h1 //and within it, at most ms_tab
            /\ HST.witnessed (HST.region_contains_pred w.region) //and the writer's region is witnessed to exists also
-           /\ HST.witnessed (MM.contains ms_tab i w) //and the writer is witnessed to be in ms_tab
+           /\ HST.witnessed (MDM.contains ms_tab i w) //and the writer is witnessed to be in ms_tab
            /\ (let old_ms = HS.sel h0 ms_tab in
               let new_ms = HS.sel h1 ms_tab in
                old_ms == new_ms //either ms_tab didn't change at all
-               \/ (MM.sel old_ms i == None
-                  /\ new_ms == MM.upd old_ms i w //or we just added w to it
+               \/ (MDM.sel old_ms i == None
+                  /\ new_ms == MDM.upd old_ms i w //or we just added w to it
                   /\ (TLSInfo.authId i ==> HS.sel h1 (AE.ilog w.log) == Seq.createEmpty))))) //and it is a fresh log
   = HST.recall ms_tab;
-    match MM.lookup ms_tab i with
+    match MDM.lookup ms_tab i with
     | None ->
       all_ms_tab_regions_exists ();
       let w = AE.gen r i in
       let wr = HST.witness_region w.region in //witness that it always exists
-      MM.extend ms_tab i w;
+      MDM.extend ms_tab i w;
       w
     | Some w ->
       N.testify (nonce_of_id i) r;   // n i -> r
