src/tls/Standalone.fst
@@ -2,12 +2,12 @@ module Standalone
 
 open FStar.Bytes
 
-module MM = FStar.Monotonic.DependentMap
+module MDM = FStar.Monotonic.DependentMap
 module HS = FStar.HyperStack
 module HST = FStar.HyperStack.ST
 
 assume val some_region : HS.rid
 type random = lbytes 32
-let injective (n:MM.partial_dependent_map random (fun _ -> HS.rid)) = True
-let nonce_rid_table : MM.t some_region random (fun _ -> HST.ex_rid) injective =
-    MM.alloc ()
+let injective (n:MDM.partial_dependent_map random (fun _ -> HS.rid)) = True
+let nonce_rid_table : MDM.t some_region random (fun _ -> HST.ex_rid) injective =
+    MDM.alloc ()
